Add facts about seq length to conversions

Sequences/NatSeqConversions.dfy
@@ -2,109 +2,135 @@ include "NatSeq.dfy"
 
 abstract module NatSeqConversions refines NatSeq {
 
-  import NatSeq1
-  import NatSeq2
+  import SmallBound
+  import LargeBound
 
-  /* NatSeq2.BASE() to the power of E() is NatSeq1.BASE(). */
-  function E(): nat
+  /* SmallBound.BOUND() to the power of E() is LargeBound.BOUND(). */
+  function method E(): nat
+    ensures power(SmallBound.BOUND(), E()) == LargeBound.BOUND()
   {
-    var n: nat :| NatSeq1.BASE() == power(NatSeq2.BASE(), n) && n > 1;
-    n
+    lemma_div_basics_auto();
+    lemma_power_multiplies_auto();
+    lemma_fundamental_div_mod(LargeBound.BITS(), SmallBound.BITS());
+    LargeBound.BITS() / SmallBound.BITS()
   }
 
-  /* Converts a sequence from NatSeq1.BASE() to NatSeq2.BASE(). */
-  function {:opaque} to_lower_base(xs: seq<NatSeq1.uint>): seq<NatSeq2.uint>
+  lemma lemma_mod_eq_zero(x: nat, y: nat)
+    requires x > 0 && y > 0
+    requires x % y == 0
+    ensures x >= y
   {
-    if |xs| == 0 then []
-    else NatSeq2.to_seq_with_len(first(xs), E()) + to_lower_base(drop_first(xs))
+    calc ==> {
+      x < y;
+        { lemma_small_mod(x, y); }
+      x % y == x;
+      false;
+    }
   }
 
-  /* Converts a sequence from NatSeq2.BASE() to NatSeq1.BASE(). */
-  function {:opaque} to_higher_base(xs: seq<NatSeq2.uint>): seq<NatSeq1.uint>
+  /* Converts a sequence from LargeBound.BOUND() to SmallBound.BOUND(). */
+  function method {:opaque} to_smaller_base(xs: seq<LargeBound.uint>): (ys: seq<SmallBound.uint>)
+    ensures |ys| == |xs| * E()
   {
     if |xs| == 0 then []
     else
-      if |xs| < E() then
-        NatSeq2.lemma_seq_nat_bound(xs);
-        lemma_power_strictly_increases(NatSeq2.BASE(), |xs|, E());
-        [NatSeq2.to_nat(xs) as NatSeq1.uint]
-      else
-        NatSeq2.lemma_seq_nat_bound(xs[..E()]);
-        lemma_mod_sub_multiples_vanish_auto();
-        [NatSeq2.to_nat(xs[..E()]) as NatSeq1.uint] + to_higher_base(xs[E()..])
+      lemma_mul_is_distributive_add_other_way(E(), 1, |xs| - 1);
+      SmallBound.from_nat_with_len(first(xs), E()) + to_smaller_base(drop_first(xs))
   }
 
-  /* Sequence conversion from NatSeq1.BASE() to NatSeq2.BASE() does not change
-  its nat representation. */
-  lemma lemma_lower_base_to_nat(xs: seq<NatSeq1.uint>)
-    ensures NatSeq2.to_nat(to_lower_base(xs)) == NatSeq1.to_nat(xs)
+  /* Converts a sequence from SmallBound.BOUND() to LargeBound.BOUND(). */
+  function method {:opaque} to_larger_base(xs: seq<SmallBound.uint>): (ys: seq<LargeBound.uint>)
+    requires |xs| % E() == 0
+    ensures |ys| == |xs| / E()
   {
-    reveal NatSeq1.to_nat();
-    reveal NatSeq2.to_nat();
-    reveal to_lower_base();
+    if |xs| == 0 then lemma_div_basics_auto(); []
+    else
+      lemma_mod_eq_zero(|xs|, E());
+      assert |xs| >= E();
+
+      SmallBound.lemma_seq_nat_bound(xs[..E()]);
+      lemma_mod_sub_multiples_vanish_auto();
+      lemma_div_minus_one(|xs|, E());
+      [SmallBound.to_nat(xs[..E()]) as LargeBound.uint] + to_larger_base(xs[E()..])
+  }
+
+  /* Sequence conversion from LargeBound.BOUND() to SmallBound.BOUND() does not
+  change its nat representation. */
+  lemma lemma_smaller_base_to_nat(xs: seq<LargeBound.uint>)
+    ensures SmallBound.to_nat(to_smaller_base(xs)) == LargeBound.to_nat(xs)
+  {
+    reveal LargeBound.to_nat();
+    reveal SmallBound.to_nat();
+    reveal to_smaller_base();
     if |xs| > 0 {
       calc {
-        NatSeq2.to_nat(to_lower_base(xs));
-        NatSeq2.to_nat(NatSeq2.to_seq_with_len(first(xs), E()) + to_lower_base(drop_first(xs)));
-          { NatSeq2.lemma_seq_prefix(NatSeq2.to_seq_with_len(first(xs), E()) + to_lower_base(drop_first(xs)), E()); }
-        NatSeq2.to_nat(NatSeq2.to_seq_with_len(first(xs), E())) + NatSeq2.to_nat(to_lower_base(drop_first(xs))) * power(NatSeq2.BASE(), E());
+        SmallBound.to_nat(to_smaller_base(xs));
+        SmallBound.to_nat(SmallBound.from_nat_with_len(first(xs), E()) + to_smaller_base(drop_first(xs)));
+          { SmallBound.lemma_seq_prefix(SmallBound.from_nat_with_len(first(xs), E()) + to_smaller_base(drop_first(xs)), E()); }
+        SmallBound.to_nat(SmallBound.from_nat_with_len(first(xs), E())) + SmallBound.to_nat(to_smaller_base(drop_first(xs))) * power(SmallBound.BOUND(), E());
           {
-            NatSeq2.lemma_to_seq_with_len_eq_to_seq(first(xs), E());
-            NatSeq2.lemma_nat_seq_nat(first(xs));
-            lemma_lower_base_to_nat(drop_first(xs));
+            SmallBound.lemma_from_nat_with_len_eq_from_nat(first(xs), E());
+            SmallBound.lemma_nat_seq_nat(first(xs));
+            lemma_smaller_base_to_nat(drop_first(xs));
           }
-        first(xs) + NatSeq1.to_nat(drop_first(xs)) * power(NatSeq2.BASE(), E());
-          { assert power(NatSeq2.BASE(), E()) == NatSeq1.BASE(); }
-        NatSeq1.to_nat(xs);
+        first(xs) + LargeBound.to_nat(drop_first(xs)) * power(SmallBound.BOUND(), E());
+          { assert power(SmallBound.BOUND(), E()) == LargeBound.BOUND(); }
+        LargeBound.to_nat(xs);
       }
     }
   }
 
-  /* Sequence conversion from NatSeq2.BASE() to NatSeq1.BASE() does not change
-  its nat representation. */
-  lemma lemma_higher_base_to_nat(xs: seq<NatSeq2.uint>)
-    ensures NatSeq1.to_nat(to_higher_base(xs)) == NatSeq2.to_nat(xs)
+  /* Sequence conversion from SmallBound.BOUND() to LargeBound.BOUND() does not
+  change its nat representation. */
+  lemma lemma_larger_base_to_nat(xs: seq<SmallBound.uint>)
+    requires |xs| % E() == 0
+    ensures LargeBound.to_nat(to_larger_base(xs)) == SmallBound.to_nat(xs)
   {
-    reveal NatSeq1.to_nat();
-    reveal NatSeq2.to_nat();
-    reveal to_higher_base();
-    if |xs| >= E() {
+    reveal LargeBound.to_nat();
+    reveal SmallBound.to_nat();
+    reveal to_larger_base();
+    if |xs| > 0 {
       calc {
-        NatSeq1.to_nat(to_higher_base(xs));
-          { NatSeq2.lemma_seq_nat_bound(xs[..E()]); }
-        NatSeq1.to_nat([NatSeq2.to_nat(xs[..E()]) as NatSeq1.uint] + to_higher_base(xs[E()..]));
-          { lemma_higher_base_to_nat(xs[E()..]); }
-        NatSeq2.to_nat(xs[..E()]) + NatSeq2.to_nat(xs[E()..]) * power(NatSeq2.BASE(), E());
-          { NatSeq2.lemma_seq_prefix(xs, E()); }
-        NatSeq2.to_nat(xs);
+        LargeBound.to_nat(to_larger_base(xs));
+          {
+            lemma_mod_eq_zero(|xs|, E());
+            lemma_mod_sub_multiples_vanish_auto();
+            SmallBound.lemma_seq_nat_bound(xs[..E()]);
+          }
+        LargeBound.to_nat([SmallBound.to_nat(xs[..E()]) as LargeBound.uint] + to_larger_base(xs[E()..]));
+          { lemma_larger_base_to_nat(xs[E()..]); }
+        SmallBound.to_nat(xs[..E()]) + SmallBound.to_nat(xs[E()..]) * power(SmallBound.BOUND(), E());
+          { SmallBound.lemma_seq_prefix(xs, E()); }
+        SmallBound.to_nat(xs);
       }
     }
   }
 
-  /* to_lower_base is injective. */
-  lemma lemma_to_lower_base_is_injective(xs: seq<NatSeq1.uint>,
-                                         ys: seq<NatSeq1.uint>)
-    requires to_lower_base(xs) == to_lower_base(ys)
+  /* to_smaller_base is injective. */
+  lemma lemma_to_smaller_base_is_injective(xs: seq<LargeBound.uint>,
+                                         ys: seq<LargeBound.uint>)
+    requires to_smaller_base(xs) == to_smaller_base(ys)
     requires |xs| == |ys|
     ensures xs == ys
   {
-    lemma_lower_base_to_nat(xs);
-    lemma_lower_base_to_nat(ys);
-    assert NatSeq1.to_nat(xs) == NatSeq1.to_nat(ys);
-    NatSeq1.lemma_seq_eq(xs, ys);
+    lemma_smaller_base_to_nat(xs);
+    lemma_smaller_base_to_nat(ys);
+    assert LargeBound.to_nat(xs) == LargeBound.to_nat(ys);
+    LargeBound.lemma_seq_eq(xs, ys);
   }
 
-  /* to_higher_base is injective. */
-  lemma lemma_to_higher_base_is_injective(xs: seq<NatSeq2.uint>,
-                                          ys: seq<NatSeq2.uint>)
-    requires to_higher_base(xs) == to_higher_base(ys)
+  /* to_larger_base is injective. */
+  lemma lemma_to_larger_base_is_injective(xs: seq<SmallBound.uint>,
+                                          ys: seq<SmallBound.uint>)
+    requires |xs| % E() == |ys| % E() == 0 
+    requires to_larger_base(xs) == to_larger_base(ys)
     requires |xs| == |ys|
     ensures xs == ys
   {
-    lemma_higher_base_to_nat(xs);
-    lemma_higher_base_to_nat(ys);
-    assert NatSeq2.to_nat(xs) == NatSeq2.to_nat(ys);
-    NatSeq2.lemma_seq_eq(xs, ys);
+    lemma_larger_base_to_nat(xs);
+    lemma_larger_base_to_nat(ys);
+    assert SmallBound.to_nat(xs) == SmallBound.to_nat(ys);
+    SmallBound.lemma_seq_eq(xs, ys);
   }
 
 }
